\noindent1. Stirling's Formula
\begin{align}
    \nonumber \sqrt{2\pi}n^{n+\frac{1}{2}}e^{-n}e^{\frac{1}{12n+1}}\textless n! \textless \sqrt{2\pi}n^{n+\frac{1}{2}}e^{-n}e^{\frac{1}{12n}} 
\end{align}
2. Transform $\frac{n}{n-x}^{\frac{n-x}{x}}$ to $e$ by using LHS\\
$\frac{n}{n-x}=\frac{n-x+x}{n-x}=1+\frac{x}{n-x}=1+\frac{1}{\frac{n-x}{x}}$\\
$\frac{n}{n-x}^{\frac{n-x}{x}}=(1+\frac{1}{\frac{n-x}{x}})^{\frac{n-x}{x}} \textless e$\\
Further more, $(\frac{n}{n-x})^{n-x} \textless e^{x}$
\begin{align}
    \nonumber (1+\frac{1}{x})^{x} \textless e \textless (1+\frac{1}{x})^{x+1}
\end{align}
3. For all real number $x$ transform $1-x$ or $1+x$ to $x$
\begin{align}
    \nonumber 1-x \le e^{-x}\\
    \nonumber 1+x \le e^{x}
\end{align}